Equations

(1)

\begin{aligned}S_{b}\left( \alpha \right) =L1\left\{ \dfrac{1}{\lambda _{1}}[ \cos \gamma _{0}-\sqrt{ 1-\lambda _{1}^{2}( 1-\cos ^{2}\alpha ] }-\cos \left( \gamma _{0}+\alpha \right) +\cos \gamma _{0}\right\} \\ .\end{aligned}

(2)

S_{0}\left( \alpha \right) =L3\left\{ \left[ \cos \left( \theta +\gamma _{0}\right) -\cos \left( \theta +\gamma _{0}+\alpha \right) \right] -\dfrac{1}{\lambda _{2}}\left( \cos \psi _{0}\right) \right\}

(3)

M_{s}\left( \alpha \right) =\dfrac{S_{b}\left( \alpha \right) }{S_{0}\left( \alpha \right) }
